theories/LambdaWt/WtTactic.v
@@ -1,0 +1,177 @@
+Require Import Coq.Lists.List.
+Require Import MirrorCore.LambdaWt.WtExpr.
+Require Import MirrorCore.LambdaWt.SubstWt.
+
+Section simple_dep_types.
+  Variable Tsymbol : Type.
+  Variable TsymbolD : Tsymbol -> Type@{Urefl}.
+  Variable Tsymbol_eq_dec : forall a b : Tsymbol, {a = b} + {a <> b}.
+
+  Variable Esymbol : type Tsymbol -> Type.
+  Variable EsymbolD : forall t, Esymbol t -> typeD TsymbolD t.
+
+  Section logicT.
+    Variable tyProp : type Tsymbol.
+    Variable forall_prop : forall (T : Type),
+        (T -> typeD TsymbolD tyProp) ->
+        typeD TsymbolD tyProp.
+
+
+    Fixpoint foralls_prop (ts : list (type Tsymbol))
+    : (HList.hlist (typeD TsymbolD) ts -> typeD TsymbolD tyProp) ->
+      typeD TsymbolD tyProp :=
+      match ts with
+      | nil => fun k => k HList.Hnil
+      | t :: ts => fun k =>
+        foralls_prop ts (fun vs =>
+                           forall_prop _ (fun v => k (HList.Hcons v vs)))
+      end.
+
+    Fixpoint foralls_uvar_prop (ts : list (Tuvar Tsymbol))
+    : (HList.hlist (fun tst => HList.hlist (typeD TsymbolD) (fst tst) -> typeD TsymbolD (snd tst)) ts -> Prop) ->
+      Prop :=
+      match ts with
+      | nil => fun k => k HList.Hnil
+      | t :: ts => fun k =>
+        foralls_uvar_prop ts (fun vs => forall v, k (HList.Hcons v vs))
+      end.
+
+    Variable impl_prop :
+        typeD TsymbolD tyProp ->
+        typeD TsymbolD tyProp ->
+        typeD TsymbolD tyProp.
+
+    Require Import ExtLib.Structures.Applicative.
+
+    Section impls.
+      Context {tus : list (Tuvar Tsymbol)} {tvs : list (type Tsymbol)}.
+      Fixpoint impls_prop (ts : list (exprT TsymbolD tus tvs (typeD TsymbolD tyProp)))
+               (post : exprT TsymbolD tus tvs (typeD TsymbolD tyProp))
+      : exprT TsymbolD tus tvs (typeD TsymbolD tyProp) :=
+        match ts with
+        | nil => post
+        | t :: ts =>
+          ap (ap (pure impl_prop) t) (impls_prop ts post)
+        end.
+    End impls.
+
+    Variable m : Type -> Type.
+
+    Inductive wtgoal tus tvs : Type :=
+    | wtSolved : wtgoal tus tvs
+    | wtGoal   : wtexpr Esymbol tus tvs tyProp -> wtgoal tus tvs
+    | wtConj   : wtgoal tus tvs -> wtgoal tus tvs -> wtgoal tus tvs
+    | wtHyp    : wtexpr Esymbol tus tvs tyProp -> wtgoal tus tvs -> wtgoal tus tvs
+    | wtAll    : forall t, wtgoal tus (t :: tvs) -> wtgoal tus tvs.
+
+    Definition migrator tus tus' : Type :=
+      forall ts t, Member.member (ts,t) tus' -> wtexpr Esymbol tus ts t.
+
+    Variables Pre Post : list (Tuvar Tsymbol) -> list (type Tsymbol) -> Type.
+
+    (** NOTE: [logicT] does not form a monad due to the generalization
+     **       over the indices.
+
+     **)
+    Definition logicT : Type :=
+      forall tus tvs
+        (prems : list (wtexpr Esymbol tus tvs tyProp))
+        (inst  : Inst Esymbol tus)
+        (goal  : Pre tus tvs),
+        m { tus' : _
+          & Post tus' tvs
+          * Inst Esymbol tus'
+          * migrator tus' tus }%type.
+
+
+
+    Variable PreD : forall {tus tvs}, Pre tus tvs ->
+                                      exprT TsymbolD tus tvs (typeD TsymbolD tyProp).
+    Variable PostD : forall {tus tvs}, Post tus tvs ->
+                                       exprT TsymbolD tus tvs (typeD TsymbolD tyProp).
+    Variable mD : forall T (TD : T -> Prop), m T -> Prop.
+
+    Variable tyProp_to_Prop : typeD TsymbolD tyProp -> Prop.
+    Variable Prop_to_tyProp : Prop -> typeD TsymbolD tyProp.
+
+    Definition migrator_tl {a b c} (mig : migrator a (b :: c))
+    : migrator a c :=
+      fun ts t X => mig ts t (Member.MN b X).
+
+
+    Section migrate.
+      Variable tus : list (Tuvar Tsymbol).
+      Variable pre : HList.hlist (fun tst : list (type Tsymbol) * type Tsymbol =>
+                       HList.hlist (typeD TsymbolD) (fst tst) ->
+                       typeD TsymbolD (snd tst)) tus.
+
+      Fixpoint migrate_env {tus'} {struct tus'}
+      : migrator tus tus' ->
+        HList.hlist (fun tst : list (type Tsymbol) * type Tsymbol =>
+                       HList.hlist (typeD TsymbolD) (fst tst) ->
+                       typeD TsymbolD (snd tst)) tus' :=
+        match tus' as tus'
+              return migrator tus tus' ->
+                     HList.hlist (fun tst : list (type Tsymbol) * type Tsymbol =>
+                                    HList.hlist (typeD TsymbolD) (fst tst) ->
+                                    typeD TsymbolD (snd tst)) tus'
+        with
+        | nil => fun _ => HList.Hnil
+        | (ts,t) :: tus' => fun mig =>
+          @HList.Hcons _ (fun tst : list (type Tsymbol) * type Tsymbol =>
+                            HList.hlist (typeD TsymbolD) (fst tst) ->
+                            typeD TsymbolD (snd tst))
+                       (ts,t) _
+                       (wtexprD EsymbolD (mig _ _ (Member.MZ _ _)) pre)
+                       (@migrate_env _ (migrator_tl mig))
+        end.
+
+    End migrate.
+
+    Definition logicT_spec (l : logicT) : Prop :=
+      forall tus tvs prems goal inst result,
+        l tus tvs prems inst goal = result ->
+        mD _ (fun t =>
+                let '(existT _ tus' (post, inst', trans)) := t in
+                foralls_uvar_prop tus' (fun us' =>
+                  InstD EsymbolD inst' us' ->
+                  tyProp_to_Prop
+                    (foralls_prop tvs (fun vs =>
+                       impls_prop (List.map (fun p us' vs => wtexprD EsymbolD p (migrate_env _ us' trans) vs) prems)
+                                  (fun us' vs =>
+                                     impl_prop (@PostD _ _ post us' vs)
+                                               (@PreD  _ _ goal  (migrate_env _ us' trans)  vs)) us' vs))))
+           result.
+  End logicT.
+End simple_dep_types.
+
+
+
+
+
+(*
+    Definition logicT_cps (Pre Post : _ -> _ -> Type) : Type :=
+      forall tus tvs
+        (prems : list (wtexpr Esymbol tus tvs tyProp))
+        (goal  : Pre tus tvs)
+        (inst  : Inst Esymbol tus)
+        (T : Type)
+        (success : forall tus' : _ ,
+            list (wtexpr Esymbol tus tvs tyProp) ->
+            Post tus' tvs ->
+            Inst Esymbol tus' ->
+            migrator tus tus' ->
+            m T)
+        (fail : unit -> m T),
+        m T.
+
+
+
+    Definition with_uvars tus (T : list (Tuvar Tsymbol) -> Type) : Type :=
+      Inst Esymbol tus ->
+      m { tus' : _ & T tus' * Inst Esymbol tus' *
+                     forall ts t, Member.member (ts,t) tus -> wtexpr Esymbol tus' ts t }%type.
+
+    Definition in_context tvs (T : Type) : Type :=
+        wtctxD
+*)
